\section{Mathematics}

\subsection{Trigonometry}
\subsubsection{Sum - difference identities}
\vspace{-0.6cm}
\begin{align*}
	\sin(u \pm v) &= \sin(u)\cos(v) \pm \cos(u)\sin(v) \\ 
	\cos(u \pm v) &= \cos(u)\cos(v) \mp \sin(u)\sin(v) \\ 
	\tan(u \pm v) &= \dfrac{\tan(u) \pm \tan(v)}{1 \mp \tan(u) \tan(v)}
\end{align*}

\subsubsection{Sum to product identities}
\vspace{-0.6cm}
\begin{align*}
	\cos(u) + \cos(v) &= 2\cos(\dfrac{u + v}{2}) \cos(\dfrac{u - v}{2}) \\ 
	\cos(u) - \cos(v) &= -2\sin(\dfrac{u + v}{2}) \sin(\dfrac{u - v}{2}) \\ 
	\sin(u) + \sin(v) &= 2\sin(\dfrac{u + v}{2}) \cos(\dfrac{u - v}{2}) \\ 
	\sin(u) - \sin(v) &= 2\cos(\dfrac{u + v}{2}) \sin(\dfrac{u - v}{2})
\end{align*}

\subsubsection{Product identities}
\vspace{-0.6cm}
\begin{align*}
	\cos(u)\cos(v) &= \dfrac{1}{2}[\cos(u + v) + \cos(u - v)] \\ 
	\sin(u)\sin(v) &= -\dfrac{1}{2}[\cos(u + v) - \cos(u - v)] \\ 
	\sin(u)\cos(v) &= \dfrac{1}{2}[\sin(u + v) + \sin(u - v)]
\end{align*}

\subsubsection{Double - triple angle identities}
\vspace{-0.6cm}
\begin{align*}
	\sin(2u) &= 2\sin(u)\cos(u) \\ 
	\cos(2u) &= 2\cos^2(u) - 1 = 1 - 2\sin^2(u) \\
	\tan(2u) &= \dfrac{2\tan(u)}{1-\tan^2(u)} \\ 
	\sin(3u) &= 3\sin(u) - 4\sin^3(u) \\ 
	\cos(3u) &= 4\cos^3(u) - 3\cos(u) \\ 
	\tan(3u) &= \dfrac{3\tan(u) - \tan^3(u)}{1 - 3\tan^2(u)}
\end{align*}

\subsection{Sums}
\vspace{-0.6cm}
\begin{align*}
	c^{a} + c^{a + 1} + \cdots + c^{b} &= \dfrac{c^{b + 1} - c^{a}}{c - 1},\ c \neq 1 \\
	c + 2c^{2} + \cdots + nc^{n} &= \dfrac{nc^{n + 2} - (n + 1)c^{n + 1} + c}{(c - 1)^2},\ c \neq 1 \\
	1 + 2 + 3 + \cdots + n &= \dfrac{n(n + 1)}{2} \\
	1^2 + 2^2 + 3^2 + \cdots + n^2 &= \dfrac{n(n + 1)(2n + 1)}{6} \\ 
	1^3 + 2^3 + 3^3 + \cdots + n^3 &= \left(\dfrac{n(n + 1)}{2}\right)^2 \\ 
	1^4 + 2^4 + 3^4 + \cdots + n^4 &= \dfrac{n(n + 1)(2n + 1)(3n^2 + 3n - 1)}{30} \\
	1^5 + 2^5 + 3^5 + \cdots + n^5 &= \dfrac{n^2(n + 1)^2(2n^2 + 2n - 1)}{12} \\
	1^6 + 2^6 + 3^6 + \cdots + n^6 &= \dfrac{n(n + 1)(2n + 1)(3n^4 + 6n^3 - 3n + 1)}{42} \\
	1^7 + 2^7 + 3^7 + \cdots + n^7 &= \dfrac{n^2(n + 1)^2(3n^4 + 6n^3 - n^2 - 4n + 2)}{24}
\end{align*}

% \subsection{Generating Pythagorean triples}
% \begin{wrapfigure}{r}{0.2\textwidth}
%     \centering
%     \includegraphics[width=0.12\textwidth]{mathematics/right_triangle}
% \end{wrapfigure}

% \begin{align*}
% 	a &= m^2 - n^2 \\ 
% 	b &= 2mn \\ 
% 	c &= m^2 + n^2
% \end{align*}
% Where $m$ and $n$ are positive integers and $m > n$. 